src/Language/PlutusIR/Semantics/SemanticEquivalence/Def.v
@@ -9,26 +9,22 @@ Notation beta_reduce := (beta_reduce tyname binderTyname substituteT).
 (* Note: The cases for Ty_Forall and and Ty_IFix make use of
    type substitution and beta reduction. However, Coq can then not
    guess the decreasing argument of fix anymore. *)
-Fixpoint R (T : Ty) (t1 t2 : Term) : Prop :=
-  emptyContext |-+ t1 : T /\
-  emptyContext |-+ t2 : T /\
+Fixpoint R (T : Ty) (ctx_K : partial_map Kind) (t1 t2 : Term) : Prop :=
+  (empty, ctx_K) |-+ t1 : T /\
+  (empty, ctx_K) |-+ t2 : T /\
   exists v1 v2,
     t1 ==> v1 /\
     t2 ==> v2 /\
     match T with
     | Ty_Forall X K T0 => 
-        (*
-        forall t0 T',
-          v1 = TyAbs X K t0 ->
-          v2 = TyAbs X K t0 ->
-          empty |-* T' : K ->
-          R (beta_reduce (substituteT X T' T0)) (TyInst v1 T') (TyInst v2 T')
-        *)
-        True
+        forall t0_1 t0_2,
+          v1 = TyAbs X K t0_1 ->
+          v2 = TyAbs X K t0_2 ->
+          R T0 (X |-> K ; ctx_K) t0_1 t0_2
     | Ty_Fun T1 T2 => 
         forall s1 s2,
-          R T1 s1 s2 ->
-          R T2 (Apply v1 s1) (Apply v2 s2)
+          R T1 ctx_K s1 s2 ->
+          R T2 ctx_K (Apply v1 s1) (Apply v2 s2)
     | Ty_Builtin st => 
         v1 = v2
     | Ty_IFix F T0 => 
@@ -41,58 +37,58 @@ Fixpoint R (T : Ty) (t1 t2 : Term) : Prop :=
     |_ => False
     end.
 
-Lemma R_typable_empty : forall T t1 t2,
-    R T t1 t2 ->
-    emptyContext |-+ t1 : T /\ emptyContext |-+ t2 : T.
+Lemma R_typable_emptyT : forall T ctxK t1 t2,
+    R T ctxK t1 t2 ->
+    (empty, ctxK) |-+ t1 : T /\ (empty, ctxK) |-+ t2 : T.
 Proof. intros. destruct T; destruct H as [Ht1 [Ht2 _]]; auto. Qed.
 
-Lemma R_typable_empty_1 : forall T t1 t2,
-    R T t1 t2 ->
-    emptyContext |-+ t1 : T.
-Proof. intros. destruct (R_typable_empty _ _ _ H). assumption. Qed.
+Lemma R_typable_emptyT_1 : forall T ctxK t1 t2,
+    R T ctxK t1 t2 ->
+    (empty, ctxK) |-+ t1 : T.
+Proof. intros. destruct (R_typable_emptyT _ _ _ _ H). assumption. Qed.
 
-Lemma R_typable_empty_2 : forall T t1 t2,
-    R T t1 t2 ->
-    emptyContext |-+ t2 : T.
-Proof. intros. destruct (R_typable_empty _ _ _ H). assumption. Qed.
+Lemma R_typable_emptyT_2 : forall T ctxK t1 t2,
+    R T ctxK t1 t2 ->
+    (empty, ctxK) |-+ t2 : T.
+Proof. intros. destruct (R_typable_emptyT _ _ _ _ H). assumption. Qed.
 
-Lemma R_evaluable : forall T t1 t2,
-    R T t1 t2 ->
+Lemma R_evaluable : forall T ctxK t1 t2,
+    R T ctxK t1 t2 ->
     exists v1 v2, t1 ==> v1 /\ t2 ==> v2.
 Proof. intros. destruct T; destruct H as [_ [_ [v1 [v2 [Hev1 [Hev2 _]]]]]]; eauto. Qed.
 
-Lemma R_evaluable_1 : forall T t1 t2,
-    R T t1 t2 ->
+Lemma R_evaluable_1 : forall T ctxK t1 t2,
+    R T ctxK t1 t2 ->
     exists v1, t1 ==> v1.
-Proof. intros. destruct (R_evaluable _ _ _ H) as [v1 [_ [Hev1 _]]]. eauto. Qed.
+Proof. intros. destruct (R_evaluable _ _ _ _ H) as [v1 [_ [Hev1 _]]]. eauto. Qed.
 
-Lemma R_evaluable_2 : forall T t1 t2,
-    R T t1 t2 ->
+Lemma R_evaluable_2 : forall T ctxK t1 t2,
+    R ctxK T t1 t2 ->
     exists v2, t2 ==> v2.
-Proof. intros. destruct (R_evaluable _ _ _ H) as [_ [v2 [_ Hev2]]]. eauto. Qed.
+Proof. intros. destruct (R_evaluable _ _ _ _ H) as [_ [v2 [_ Hev2]]]. eauto. Qed.
 
-Lemma R_syntactic_equality : forall st t1 t2,
-    R (Ty_Builtin st) t1 t2 ->
+Lemma R_syntactic_equality : forall st ctxK t1 t2,
+    R (Ty_Builtin st) ctxK t1 t2 ->
     exists v1 v2,
       t1 ==> v1 /\
       t2 ==> v2 /\
       v1 = v2.
 Proof. intros. destruct H as [_ [_ [v1 [v2 [Hev1 [Hev2 Heq]]]]]]. eauto. Qed.
 
-Lemma R_functional_extensionality : forall T1 T2 t1 t2,
-  R (Ty_Fun T1 T2) t1 t2 ->
+Lemma R_functional_extensionality : forall T1 T2 ctxK t1 t2,
+  R (Ty_Fun T1 T2) ctxK t1 t2 ->
   exists v1 v2,
     t1 ==> v1 /\
     t2 ==> v2 /\
     (forall s1 s2,
-      R T1 s1 s2 ->
-      R T2 (Apply v1 s1) (Apply v2 s2)).
+      R T1 ctxK s1 s2 ->
+      R T2 ctxK (Apply v1 s1) (Apply v2 s2)).
 Proof. intros. destruct H as [_ [_ [v1 [v2 [Hev1 [Hev2 Hfe]]]]]]. eauto. Qed.
 
-Lemma R_falsity : forall t1 t2,
-  (forall a, ~(R (Ty_Var a) t1 t2)) /\
-  (forall bX K T, ~(R (Ty_Lam bX K T) t1 t2)) /\
-  (forall T1 T2, ~(R (Ty_App T1 T2) t1 t2)).
+Lemma R_falsity : forall ctxK t1 t2,
+  (forall a, ~(R (Ty_Var a) ctxK t1 t2)) /\
+  (forall bX K T, ~(R (Ty_Lam bX K T) ctxK t1 t2)) /\
+  (forall T1 T2, ~(R (Ty_App T1 T2) ctxK t1 t2)).
 Proof. 
   split.
   - intros. intro Hcon. destruct Hcon as [_ [_ [_ [_ [_ [_ Hfalse]]]]]]. destruct Hfalse.
@@ -129,7 +125,7 @@ Program Fixpoint R'' (T : Ty) (t1 t2 : Term) {measure (countBindingLocations T)}
           v1 = TyAbs X K t0 ->
           v2 = TyAbs X K t0 ->
           emptyContext |-* T' : K ->
-          R'' (beta_reduce (substituteT X T' T0)) (TyInst v1 T') (TyInst v2 T')
+          R'' (Named.beta_reduce (substituteT X T' T0)) (TyInst v1 T') (TyInst v2 T')
     | Ty_Fun T1 T2 => 
         forall s1 s2,
           R'' T1 s1 s2 ->
@@ -139,7 +135,7 @@ Program Fixpoint R'' (T : Ty) (t1 t2 : Term) {measure (countBindingLocations T)}
     | Ty_IFix F T0 => 
         forall X K,
           emptyContext |-* T : K ->
-          R'' (beta_reduce (unwrapIFix F X K T0)) (Unwrap v1) (Unwrap v2)
+          R'' (Named.beta_reduce (unwrapIFix F X K T0)) (Unwrap v1) (Unwrap v2)
     |_ => False
     end.
 Next Obligation. Admitted.
@@ -165,7 +161,7 @@ Equations R' (T : Ty) (t1 t2 : Term) : Prop by wf (countBindingLocations T) :=
             v1 = TyAbs X K t0 ->
             v2 = TyAbs X K t0 ->
             emptyContext |-* T' : K ->
-            R' (beta_reduce (substituteT X T' T0)) (TyInst v1 T') (TyInst v2 T')
+            R' (Named.beta_reduce (substituteT X T' T0)) (TyInst v1 T') (TyInst v2 T')
       | Ty_Fun T1 T2 => 
           forall s1 s2,
             R' T1 s1 s2 ->
@@ -175,7 +171,7 @@ Equations R' (T : Ty) (t1 t2 : Term) : Prop by wf (countBindingLocations T) :=
       | Ty_IFix F T0 => 
           forall X K,
             emptyContext |-* T : K ->
-            R' (beta_reduce (unwrapIFix F X K T0)) (Unwrap v1) (Unwrap v2)
+            R' (Named.beta_reduce (unwrapIFix F X K T0)) (Unwrap v1) (Unwrap v2)
       |_ => False
       end.
       
@@ -205,5 +201,3 @@ with R2 : Ty -> Term -> Term -> Prop :=
         R T1 s1 s2 ->
         R T2 (Apply v1 s1) (Apply v2 s2)) ->
       R2 (Ty_Fun T1 T2) v1 v2.
-
-
